Commit some WIP.

SmtQuery.v
@@ -321,131 +321,106 @@ Proof.
   f_equal.
 Qed.
 
-Definition get_vids_from_prog (field_type : PSField) (p : CaracaraProgram) : list positive :=
-  match p with
-  | CaracaraProgramDef headers states ctrls transformer =>
-      match field_type with
-      | PSHeader => map (fun h => match h with HeaderCtr uid => uid end) headers
-      | PSState => map (fun s => match s with StateCtr uid => uid end) states
-      | PSCtrl => map (fun c => match c with CtrlCtr uid => uid end) ctrls
-      end
-  end.
+Class CrVarProg A := {
+  get_vars_from_prog : CaracaraProgram -> list A;
+  lookup_var : ConcreteState -> A -> uint8;
+  get_vars_invariant_of_transformer:
+    forall h s c t1 t2,
+    get_vars_from_prog (CaracaraProgramDef h s c t1) =
+    get_vars_from_prog (CaracaraProgramDef h s c t2);
+  equivalence_checker_cr_sound :
+    forall p1 p2 f,
+    equivalence_checker_cr_dsl p1 p2 = Equivalent ->
+    let c1_i  := eval_sym_state (init_symbolic_state p1) f in (* Get a sym state out of p1 *)
+    let c2_i  := eval_sym_state (init_symbolic_state p2) f in (* Do the same for p2 *)
+    let t1 := get_transformer_from_prog p1 in
+    let t2 := get_transformer_from_prog p2 in
+    let c1 := eval_transformer_concrete t1 c1_i in
+    let c2 := eval_transformer_concrete t2 c2_i in
+    well_formed_program p1 ->                          (* p1 is well-formed *)
+    forall var, In var (get_vars_from_prog p1) ->      (* then, every var in p1 *)
+    (In var (get_vars_from_prog p2)) /\                (* must be in p2 *)
+    (lookup_var c1 var) = (lookup_var c2 var);         (* and their final values must be equal *)
+}.
 
-Definition lookup_vid (field_type : PSField) (s : ConcreteState) (vid : positive) : uint8 :=
-  match field_type with
-  | PSHeader => lookup_varlike s (HeaderCtr vid)
-  | PSState => lookup_varlike s (StateCtr vid)
-  | PSCtrl => lookup_varlike s (CtrlCtr vid)
-  end.
-
-Lemma equivalence_checker_cr_sound :
-  forall p1 p2 f field_type,
-  field_type <> PSCtrl ->                                   (* TODO: Bit of a hack, need to fix *)
-  equivalence_checker_cr_dsl p1 p2 = Equivalent ->
-  let c1_i  := eval_sym_state (init_symbolic_state p1) f in (* Get a sym state out of p1' headers, ctrls, and state *)
-  let c2_i  := eval_sym_state (init_symbolic_state p2) f in (* Do the same for p2 *)
-  let t1 := get_transformer_from_prog p1 in
-  let t2 := get_transformer_from_prog p2 in
-  let c1 := eval_transformer_concrete t1 c1_i in
-  let c2 := eval_transformer_concrete t2 c2_i in
-  well_formed_program p1 ->                          (* p1 is well-formed *)
-  (forall vid, In vid (get_vids_from_prog field_type p1) ->      (* then, every header in p1 *)
-  (In vid (get_vids_from_prog field_type p2)) /\               (* must be in p2 *)
-  (lookup_vid field_type c1 vid) = (lookup_vid field_type c2 vid)).            (* and their final values must be equal *)
+Instance CrVarProg_Header : CrVarProg Header.
 Proof.
-  intros p1 p2 f field_type not_ctrl H.
-  destruct p1 as [h1 s1 c1 t1] eqn:desp1,
-           p2 as [h2 s2 c2 t2] eqn:desp2; simpl in H.
-  destruct
-  (varlike_list_equal h1 h2) eqn:H_hdr_eq,
-  (varlike_list_equal s1 s2) eqn:H_state_eq,
-  (varlike_list_equal c1 c2) eqn:H_ctrl_eq in H; simpl in H; try (exfalso; congruence).
-  intros.
-  simpl in H1. (* TODO: May want to remove these *)
-  split.
-  - destruct field_type eqn:ft.
-    + exfalso. apply not_ctrl. reflexivity.
-    + apply varlike_list_equal_lemma in H_hdr_eq.
-      rewrite H_hdr_eq in H1.
-      assumption.
-    + apply varlike_list_equal_lemma in H_state_eq.
-      rewrite H_state_eq in H1.
-      assumption.
-  - destruct (equivalence_checker (init_symbolic_state (CaracaraProgramDef h1 s1 c1 t1)) t1 t2 h1 s1) eqn:H_eq; try (exfalso; congruence).
+  refine {| get_vars_from_prog := get_headers_from_prog;
+            lookup_var := fun s h => lookup_varlike s h; |}.
+  - intros. simpl. reflexivity.
+  - intros p1 p2 f H.
+    destruct p1 as [h1 s1 c1 t1] eqn:desp1,
+             p2 as [h2 s2 c2 t2] eqn:desp2; simpl in H.
+    destruct
+    (varlike_list_equal h1 h2) eqn:H_hdr_eq,
+    (varlike_list_equal s1 s2) eqn:H_state_eq,
+    (varlike_list_equal c1 c2) eqn:H_ctrl_eq in H; simpl in H; try (exfalso; congruence).
+    intros.
+    simpl in H1.
+    split.
+    -- apply varlike_list_equal_lemma in H_hdr_eq.
+       rewrite H_hdr_eq in H1.
+       assumption.
+    -- destruct (equivalence_checker (init_symbolic_state (CaracaraProgramDef h1 s1 c1 t1)) t1 t2 h1 s1) eqn:H_eq; try (exfalso; congruence).
     apply equivalence_checker_sound with (f := f) in H_eq.
-    + destruct field_type eqn:ft.
-      * exfalso. apply not_ctrl. reflexivity. 
-      * simpl in H1.
-        remember (HeaderCtr vid) as v.
-        apply in_map_iff in H1.
-        destruct H1 as [h [Hin Heq]].
-        apply H_eq in Heq.
-        unfold c0.
-        unfold c3.
-        unfold c1_i.
-        unfold c2_i.
-        simpl.
-        unfold t0.
-        unfold t3.
-        simpl.
-        apply varlike_list_equal_lemma in H_state_eq.
-        apply varlike_list_equal_lemma in H_hdr_eq.
-        apply varlike_list_equal_lemma in H_ctrl_eq.
-        rewrite <- H_hdr_eq.
-        rewrite <- H_state_eq.
-        rewrite <- H_ctrl_eq.
-        rewrite init_symbolic_state_nodep_t with (t2 := t2) in Heq at 2.
-        assert (h = HeaderCtr vid). { destruct h. rewrite Hin. reflexivity. }
-        rewrite <- H1.
-        apply Heq.
-      * simpl in H1.
-        remember (StateCtr vid) as v.
-        apply in_map_iff in H1.
-        destruct H1 as [h [Hin Heq]].
-        apply H_eq in Heq.
-        unfold c0.
-        unfold c3.
-        unfold c1_i.
-        unfold c2_i.
-        simpl.
-        unfold t0.
-        unfold t3.
-        simpl.
-        apply varlike_list_equal_lemma in H_state_eq.
-        apply varlike_list_equal_lemma in H_hdr_eq.
-        apply varlike_list_equal_lemma in H_ctrl_eq.
-        rewrite <- H_hdr_eq.
-        rewrite <- H_state_eq.
-        rewrite <- H_ctrl_eq.
-        rewrite init_symbolic_state_nodep_t with (t2 := t2) in Heq at 2.
-        assert (h = StateCtr vid). { destruct h. rewrite Hin. reflexivity. }
-        rewrite <- H1.
-        apply Heq.
-    + intros.
-      apply is_varlike_in_ps_lemma.
-      unfold init_symbolic_state.
-      Transparent get_all_varlike_from_ps.
-      unfold get_all_varlike_from_ps.
-      simpl.
-      repeat rewrite map_pair_split.
-      simpl.
-      apply (@ptree_of_list_lemma_generic Header CrVarLike_Header).
-      simpl in H0.
-      destruct H0.
-      assumption. assumption.
-    + intros.
-      apply is_varlike_in_ps_lemma.
-      unfold init_symbolic_state.
-      unfold get_all_varlike_from_ps.
-      simpl.
-      repeat rewrite map_pair_split.
-      simpl.
-      apply (@ptree_of_list_lemma_generic State CrVarLike_State).
-      simpl in H0.
-      destruct H0.
-      destruct H3.
-      assumption. assumption.
-Qed.
+      ++ apply H_eq in H1.
+         unfold c0.
+         unfold c3.
+         unfold c1_i.
+         unfold c2_i.
+         simpl.
+         unfold t0.
+         unfold t3.
+         simpl.
+         apply varlike_list_equal_lemma in H_state_eq.
+         apply varlike_list_equal_lemma in H_hdr_eq.
+         apply varlike_list_equal_lemma in H_ctrl_eq.
+         rewrite <- H_hdr_eq.
+         rewrite <- H_state_eq.
+         rewrite <- H_ctrl_eq.
+         rewrite init_symbolic_state_nodep_t with (t2 := t2) in H1 at 2.
+         assumption.
+      ++ intros.
+         apply is_varlike_in_ps_lemma.
+         unfold init_symbolic_state.
+          Transparent get_all_varlike_from_ps.
+          unfold get_all_varlike_from_ps.
+          simpl.
+          repeat rewrite map_pair_split.
+          simpl.
+          apply (@ptree_of_list_lemma_generic Header CrVarLike_Header).
+          simpl in H0.
+          destruct H0.
+          assumption. assumption.
+      ++ intros.
+         apply is_varlike_in_ps_lemma.
+         unfold init_symbolic_state.
+         unfold get_all_varlike_from_ps.
+         simpl.
+         repeat rewrite map_pair_split. 
+         simpl.
+         apply (@ptree_of_list_lemma_generic State CrVarLike_State).
+         simpl in H0.
+         destruct H0.
+         destruct H3.
+         assumption. assumption.
+Defined.
+
+Instance CrVarProg_State : CrVarProg State.
+Proof.
+  refine {| get_vars_from_prog := get_states_from_prog;
+            lookup_var := fun s sv => lookup_varlike s sv; |}.
+  - intros. simpl. reflexivity.
+  - admit.
+Admitted.
+
+Instance CrVarProg_Ctrl : CrVarProg Ctrl.
+Proof.
+  refine {| get_vars_from_prog := get_ctrls_from_prog;
+            lookup_var := fun s c => lookup_varlike s c; |}.
+  - intros. simpl. reflexivity.
+  - admit.
+Admitted.
 
 Transparent map_from_ps.
 (* Completeness lemma for equivalence_checker_cr_dsl *)
